new/generatedproof/github_com/goose_lang/goose/testdata/examples/append_log.v
@@ -26,7 +26,7 @@ End Log.
 Section instances.
 Context `{ffi_syntax}.
 
-Global Instance settable_Log : Settable _ :=
+Global Instance settable_Log : Settable Log.t :=
   settable! Log.mk < Log.m'; Log.sz'; Log.diskSz' >.
 Global Instance into_val_Log : IntoVal Log.t :=
   {| to_val_def v :=
