new/generatedproof/github_com/mit_pdos/go_journal/buf.v
@@ -29,7 +29,7 @@ End Buf.
 Section instances.
 Context `{ffi_syntax}.
 
-Global Instance settable_Buf : Settable _ :=
+Global Instance settable_Buf : Settable Buf.t :=
   settable! Buf.mk < Buf.Addr'; Buf.Sz'; Buf.Data'; Buf.dirty' >.
 Global Instance into_val_Buf : IntoVal Buf.t :=
   {| to_val_def v :=
@@ -111,7 +111,7 @@ End BufMap.
 Section instances.
 Context `{ffi_syntax}.
 
-Global Instance settable_BufMap : Settable _ :=
+Global Instance settable_BufMap : Settable BufMap.t :=
   settable! BufMap.mk < BufMap.addrs' >.
 Global Instance into_val_BufMap : IntoVal BufMap.t :=
   {| to_val_def v :=
